Lp2lc/Active/DTLC/Proof.lean
@@ -1,0 +1,25 @@
+import Std
+import «Lp2lc».Active.Shared
+import «Lp2lc».Active.Util
+import «Lp2lc».Active.DTLC.Def
+
+namespace Lp2lc.Active
+
+namespace DTLC
+
+namespace Trm
+
+open Util
+
+/-- Erasing annotations always produces a type-erased term. -/
+theorem eraseType_isErased (I : Index) : ∀ (self : Trm I), self.typeEraseAll.TypeIsErased
+| .val (.primitive _) _ => rfl
+| .val (.fn body _) _ =>
+  ⟨rfl, rfl, fun arg => eraseType_isErased I (body arg)⟩
+| .apply fn arg _ =>
+  ⟨rfl, eraseType_isErased I fn, eraseType_isErased I arg⟩
+| .ref _ _ => rfl
+
+end Trm
+
+end DTLC
